src/verified_adapter.mli
@@ -9,3 +9,4 @@ val convert_violations: (Verified.Monitor.nat * Predicate.cst option list) Verif
 val domain_ceq: cst Verified.Monitor.ceq
 val domain_ccompare: cst Verified.Monitor.ccompare
 val domain_equal: cst Verified.Monitor.equal
+val domain_set_impl: cst Verified.Monitor.set_impl
